theories/Syntax/Term.v
@@ -1,34 +1,405 @@
-From Stdlib Require Import List Utf8.
+From Stdlib Require Import List Arith Lia Utf8 FunctionalExtensionality Wellfounded Program.Equality.
+From Stdlib.Vectors Require Import Fin Vector.
 
 From Cyclic.Syntax Require Import StrictPos.
 
-Import StrictPos.
 Import ListNotations.
 
 Set Default Proof Using "Type".
 
-(* Raw (untyped) syntax for a CoC-style dependent calculus with general recursion
-   and inductive data (given by strictly-positive signatures).
-
-   This is intentionally lightweight: typing, conversion, and operational
-   semantics will live in separate files.
-
-   We use de Bruijn indices for binders.
-*)
-
 Module Syntax.
-  Inductive ty : Type :=
-  | TyU
-  | TyPi (A : ty) (B : ty) (* B lives in extended context *)
-  | TyInd (Σ : ind_sig ty).
-
   Inductive tm : Type :=
   | tVar (x : nat)
-  | tLam (A : ty) (t : tm)
+  | tSort (i : nat)
+  | tPi (A : tm) (B : tm)
+  | tLam (A : tm) (t : tm)
   | tApp (t u : tm)
-  | tFix (A : ty) (t : tm) (* t is in extended context, binds the recursive name *)
-  | tRoll (Σ : ind_sig ty) (s : Shape Σ)
-      (params : ParamPos Σ s -> tm)
-      (k : Pos Σ s -> tm)
-  | tCase (Σ : ind_sig ty) (scrut : tm) (C : ty) (br : Shape Σ -> tm).
+  | tFix (A : tm) (t : tm)
+  | tInd (I : nat)
+  | tRoll (I : nat) (c : nat) (params recs : list tm)
+  | tCase (I : nat) (n : nat) (scrut : tm) (C : tm) (brs : Vector.t tm n).
+
+  Definition branch {n} (brs : Vector.t tm n) (k : Fin.t n) : tm :=
+    Vector.nth brs k.
+
+  Fixpoint shift (d : nat) (c : nat) (t : tm) : tm :=
+    match t with
+    | tVar x => if Nat.ltb x c then tVar x else tVar (x + d)
+    | tSort i => tSort i
+    | tPi A B => tPi (shift d c A) (shift d (S c) B)
+    | tLam A t => tLam (shift d c A) (shift d (S c) t)
+    | tApp t u => tApp (shift d c t) (shift d c u)
+    | tFix A t => tFix (shift d c A) (shift d (S c) t)
+    | tInd ind => tInd ind
+    | tRoll ind ctor ps rs =>
+        tRoll ind ctor (List.map (shift d c) ps) (List.map (shift d c) rs)
+    | tCase ind n scrut C brs =>
+        tCase ind n (shift d c scrut) (shift d c C) (Vector.map (shift d c) brs)
+    end.
+
+  Definition up (σ : nat -> tm) : nat -> tm :=
+    fun x => match x with 0 => tVar 0 | S x => shift 1 0 (σ x) end.
+
+  Fixpoint subst (σ : nat -> tm) (t : tm) : tm :=
+    match t with
+    | tVar x => σ x
+    | tSort i => tSort i
+    | tPi A B => tPi (subst σ A) (subst (up σ) B)
+    | tLam A t => tLam (subst σ A) (subst (up σ) t)
+    | tApp t u => tApp (subst σ t) (subst σ u)
+    | tFix A t => tFix (subst σ A) (subst (up σ) t)
+    | tInd ind => tInd ind
+    | tRoll ind ctor ps rs =>
+        tRoll ind ctor (List.map (subst σ) ps) (List.map (subst σ) rs)
+    | tCase ind n scrut C brs =>
+        tCase ind n (subst σ scrut) (subst σ C) (Vector.map (subst σ) brs)
+    end.
+
+  Definition subst0 (u : tm) (t : tm) : tm :=
+    subst (fun x => match x with 0 => u | S x => tVar x end) t.
+
+  Module Lemmas.
+    Fixpoint sum_list (ns : list nat) : nat :=
+      match ns with
+      | [] => 0
+      | n :: ns => n + sum_list ns
+      end.
+
+    Fixpoint sum_fin (n : nat) (f : Fin.t n -> nat) : nat :=
+      match n as n0 return (Fin.t n0 -> nat) -> nat with
+      | 0 => fun _ => 0
+      | S n => fun f => f Fin.F1 + sum_fin n (fun k => f (Fin.FS k))
+      end f.
+
+    Fixpoint size (t : tm) : nat :=
+      match t with
+      | tVar _ => 1
+      | tSort _ => 1
+      | tPi A B => 1 + size A + size B
+      | tLam A t => 1 + size A + size t
+      | tApp t u => 1 + size t + size u
+      | tFix A t => 1 + size A + size t
+      | tInd _ => 1
+      | tRoll _ _ ps rs => 1 + sum_list (List.map size ps) + sum_list (List.map size rs)
+      | tCase _ n scrut C brs =>
+          1 + size scrut + size C + sum_fin n (fun k => size (branch brs k))
+      end.
+
+    Definition wf_tm : well_founded (fun t1 t2 => size t1 < size t2) :=
+      wf_inverse_image _ _ lt size Nat.lt_wf_0.
+
+    Lemma size_lt_roll_param {I c} {params recs : list tm} {p : tm} :
+      List.In p params -> size p < size (tRoll I c params recs).
+    Proof.
+      intro Hin.
+      simpl.
+      pose proof (size_le_sum_list (ps:=params) (p:=p) Hin) as Hle.
+      lia.
+    Qed.
+
+    Lemma size_lt_roll_rec {I c} {params recs : list tm} {r : tm} :
+      List.In r recs -> size r < size (tRoll I c params recs).
+    Proof.
+      intro Hin.
+      simpl.
+      pose proof (size_le_sum_list (ps:=recs) (p:=r) Hin) as Hle.
+      lia.
+    Qed.
+
+    Lemma size_le_sum_list {ps : list tm} {p : tm} :
+      List.In p ps -> size p <= sum_list (List.map size ps).
+    Proof.
+      intro Hin.
+      induction ps as [|q qs IH]; simpl in *.
+      - contradiction.
+      - destruct Hin as [Hin|Hin]; subst.
+        + lia.
+        + specialize (IH Hin).
+          lia.
+    Qed.
+
+    Lemma size_lt_case_branch {I n} {scrut C : tm} {brs : Vector.t tm n} (k : Fin.t n) :
+      size (branch brs k) < size (tCase I n scrut C brs).
+    Proof.
+      simpl.
+      pose proof (size_le_sum_fin brs k) as Hle.
+      lia.
+    Qed.
+
+    Lemma size_le_sum_fin {n} (brs : Vector.t tm n) (k : Fin.t n) :
+      size (branch brs k) <= sum_fin n (fun j => size (branch brs j)).
+    Proof.
+      revert brs k.
+      induction n as [|n IH]; intros brs k.
+      - inversion k.
+      - dependent destruction brs.
+        dependent destruction k.
+        + simpl. lia.
+        + simpl.
+          specialize (IH brs k).
+          lia.
+    Qed.
+
+    Definition shift_sub (d c : nat) : nat -> tm :=
+      fun x => if Nat.ltb x c then tVar x else tVar (x + d).
+
+    Lemma up_shift_sub d c : up (shift_sub d c) = shift_sub d (S c).
+    Proof.
+      apply functional_extensionality; intro x.
+      destruct x as [|x]; simpl.
+      - reflexivity.
+      - unfold shift_sub.
+        destruct (Nat.ltb x c) eqn:Hlt.
+        + apply Nat.ltb_lt in Hlt.
+          assert (Nat.ltb (S x) (S c) = true) as Hlt'.
+          { apply Nat.ltb_lt. lia. }
+          rewrite Hlt'.
+          simpl.
+          f_equal.
+          lia.
+        + apply Nat.ltb_ge in Hlt.
+          assert (Nat.ltb (S x) (S c) = false) as Hge'.
+          { apply Nat.ltb_ge. lia. }
+          rewrite Hge'.
+          simpl.
+          f_equal.
+          lia.
+    Qed.
+
+    Lemma up_ext (σ τ : nat -> tm) :
+      (forall x, σ x = τ x) -> forall x, up σ x = up τ x.
+    Proof.
+      intro Heq.
+      intro x.
+      destruct x as [|x]; simpl; [reflexivity|].
+      rewrite Heq.
+      reflexivity.
+    Qed.
+
+    Lemma subst_ext (σ τ : nat -> tm) (t : tm) :
+      (forall x, σ x = τ x) -> subst σ t = subst τ t.
+    Proof.
+      intro Heq.
+      revert σ τ Heq.
+      refine (Wf.well_founded_induction _ _ wf_tm
+        (fun t => forall σ τ, (forall x, σ x = τ x) -> subst σ t = subst τ t)
+        _ t).
+      intros t0 IH σ τ Heq0.
+      destruct t0 as
+        [x|i|A B|A body|fn arg|A body|ind|ind ctor params recs|ind n scrut C brs];
+        simpl; try reflexivity.
+      - exact (Heq0 x).
+      - f_equal.
+        + apply (IH A). simpl; lia. exact σ. exact τ. exact Heq0.
+        + apply (IH B). simpl; lia. exact (up σ). exact (up τ).
+          exact (up_ext _ _ Heq0).
+      - f_equal.
+        + apply (IH A). simpl; lia. exact σ. exact τ. exact Heq0.
+        + apply (IH body). simpl; lia. exact (up σ). exact (up τ).
+          exact (up_ext _ _ Heq0).
+      - f_equal.
+        + apply (IH fn). simpl; lia. exact σ. exact τ. exact Heq0.
+        + apply (IH arg). simpl; lia. exact σ. exact τ. exact Heq0.
+      - f_equal.
+        + apply (IH A). simpl; lia. exact σ. exact τ. exact Heq0.
+        + apply (IH body). simpl; lia. exact (up σ). exact (up τ).
+          exact (up_ext _ _ Heq0).
+      - f_equal.
+        + apply List.map_ext_in.
+          intros p Hp.
+          apply (IH p).
+          * apply size_lt_roll_param; exact Hp.
+          * exact σ.
+          * exact τ.
+          * exact Heq0.
+        + apply List.map_ext_in.
+          intros r Hr.
+          apply (IH r).
+          * apply size_lt_roll_rec; exact Hr.
+          * exact σ.
+          * exact τ.
+          * exact Heq0.
+      - f_equal.
+        + apply (IH scrut). simpl; lia. exact σ. exact τ. exact Heq0.
+        + apply (IH C). simpl; lia. exact σ. exact τ. exact Heq0.
+        + apply Vector.map_ext.
+          intro k.
+          apply (IH (branch brs k)).
+          * apply size_lt_case_branch.
+          * exact σ.
+          * exact τ.
+          * exact Heq0.
+    Qed.
+
+    Lemma shift_as_subst (d c : nat) (t : tm) :
+      shift d c t = subst (shift_sub d c) t.
+    Proof.
+      revert c.
+      refine (Wf.well_founded_induction _ _ wf_tm
+        (fun t => forall c, shift d c t = subst (shift_sub d c) t)
+        _ t).
+      intros t0 IH c0.
+      destruct t0 as
+        [x|i|A B|A body|fn arg|A body|ind|ind ctor params recs|ind n scrut C brs];
+        simpl; try reflexivity.
+      - unfold shift_sub.
+        destruct (Nat.ltb x c0); reflexivity.
+      - f_equal.
+        + apply (IH A). simpl; lia. exact c0.
+        + rewrite (IH B). 2: (simpl; lia). 2: exact (S c0).
+          rewrite up_shift_sub.
+          reflexivity.
+      - f_equal.
+        + apply (IH A). simpl; lia. exact c0.
+        + rewrite (IH body). 2: (simpl; lia). 2: exact (S c0).
+          rewrite up_shift_sub.
+          reflexivity.
+      - f_equal.
+        + apply (IH fn). simpl; lia. exact c0.
+        + apply (IH arg). simpl; lia. exact c0.
+      - f_equal.
+        + apply (IH A). simpl; lia. exact c0.
+        + rewrite (IH body). 2: (simpl; lia). 2: exact (S c0).
+          rewrite up_shift_sub.
+          reflexivity.
+      - f_equal.
+        + apply List.map_ext_in.
+          intros p Hp.
+          apply (IH p).
+          * apply size_lt_roll_param; exact Hp.
+          * exact c0.
+        + apply List.map_ext_in.
+          intros r Hr.
+          apply (IH r).
+          * apply size_lt_roll_rec; exact Hr.
+          * exact c0.
+      - f_equal.
+        + apply (IH scrut). simpl; lia. exact c0.
+        + apply (IH C). simpl; lia. exact c0.
+        + apply Vector.map_ext.
+          intro k.
+          apply (IH (branch brs k)).
+          * apply size_lt_case_branch.
+          * exact c0.
+    Qed.
+
+    Lemma subst_shift0 (σ : nat -> tm) (t : tm) :
+      subst (up σ) (shift 1 0 t) = shift 1 0 (subst σ t).
+    Proof.
+      revert σ.
+      refine (Wf.well_founded_induction _ _ wf_tm
+        (fun t => forall σ, subst (up σ) (shift 1 0 t) = shift 1 0 (subst σ t))
+        _ t).
+      intros t0 IH σ.
+      destruct t0 as
+        [x|i|A B|A body|fn arg|A body|ind|ind ctor params recs|ind n scrut C brs];
+        simpl; try reflexivity.
+      - destruct (Nat.ltb x 0) eqn:Hlt.
+        + apply Nat.ltb_lt in Hlt; lia.
+        + destruct x as [|x]; simpl.
+          * reflexivity.
+          * rewrite Nat.add_1_r.
+            reflexivity.
+      - f_equal.
+        + apply (IH A). simpl; lia. exact σ.
+        + apply (IH B). simpl; lia. exact (up σ).
+      - f_equal.
+        + apply (IH A). simpl; lia. exact σ.
+        + apply (IH body). simpl; lia. exact (up σ).
+      - f_equal.
+        + apply (IH fn). simpl; lia. exact σ.
+        + apply (IH arg). simpl; lia. exact σ.
+      - f_equal.
+        + apply (IH A). simpl; lia. exact σ.
+        + apply (IH body). simpl; lia. exact (up σ).
+      - f_equal.
+        + apply List.map_ext_in.
+          intros p Hp.
+          apply (IH p).
+          * apply size_lt_roll_param; exact Hp.
+          * exact σ.
+        + apply List.map_ext_in.
+          intros r Hr.
+          apply (IH r).
+          * apply size_lt_roll_rec; exact Hr.
+          * exact σ.
+      - f_equal.
+        + apply (IH scrut). simpl; lia. exact σ.
+        + apply (IH C). simpl; lia. exact σ.
+        + apply Vector.map_ext.
+          intro k.
+          apply (IH (branch brs k)).
+          * apply size_lt_case_branch.
+          * exact σ.
+    Qed.
+
+    Lemma up_comp_subst (σ τ : nat -> tm) :
+      forall x, up (fun y => subst σ (τ y)) x = subst (up σ) (up τ x).
+    Proof.
+      intro x.
+      destruct x as [|x]; simpl; [reflexivity|].
+      symmetry.
+      apply (subst_shift0 σ (τ x)).
+    Qed.
+
+    Lemma subst_comp (σ τ : nat -> tm) (t : tm) :
+      subst σ (subst τ t) = subst (fun x => subst σ (τ x)) t.
+    Proof.
+      revert σ τ.
+      refine (Wf.well_founded_induction _ _ wf_tm
+        (fun t => forall σ τ,
+          subst σ (subst τ t) = subst (fun x => subst σ (τ x)) t)
+        _ t).
+      intros t0 IH σ τ.
+      destruct t0 as
+        [x|i|A B|A body|fn arg|A body|ind|ind ctor params recs|ind n scrut C brs];
+        simpl; try reflexivity.
+      - f_equal.
+        + apply (IH A). simpl; lia. exact σ. exact τ.
+        + rewrite (IH B). 2: (simpl; lia). 2: exact (up σ). 2: exact (up τ).
+          apply subst_ext.
+          intro x.
+          symmetry.
+          apply up_comp_subst.
+      - f_equal.
+        + apply (IH A). simpl; lia. exact σ. exact τ.
+        + rewrite (IH body). 2: (simpl; lia). 2: exact (up σ). 2: exact (up τ).
+          apply subst_ext.
+          intro x.
+          symmetry.
+          apply up_comp_subst.
+      - f_equal.
+        + apply (IH fn). simpl; lia. exact σ. exact τ.
+        + apply (IH arg). simpl; lia. exact σ. exact τ.
+      - f_equal.
+        + apply (IH A). simpl; lia. exact σ. exact τ.
+        + rewrite (IH body). 2: (simpl; lia). 2: exact (up σ). 2: exact (up τ).
+          apply subst_ext.
+          intro x.
+          symmetry.
+          apply up_comp_subst.
+      - f_equal.
+        + apply List.map_ext_in.
+          intros p Hp.
+          apply (IH p).
+          * apply size_lt_roll_param; exact Hp.
+          * exact σ.
+          * exact τ.
+        + apply List.map_ext_in.
+          intros r Hr.
+          apply (IH r).
+          * apply size_lt_roll_rec; exact Hr.
+          * exact σ.
+          * exact τ.
+      - f_equal.
+        + apply (IH scrut). simpl; lia. exact σ. exact τ.
+        + apply (IH C). simpl; lia. exact σ. exact τ.
+        + apply Vector.map_ext.
+          intro k.
+          apply (IH (branch brs k)).
+          * apply size_lt_case_branch.
+          * exact σ.
+          * exact τ.
+    Qed.
+  End Lemmas.
 End Syntax.
